theories/L/Complexity/Reductions/Cook/tmp.v
@@ -1,0 +1,8 @@
+Require Import Lia.
+
+Goal forall n, n < 5 -> exists X, n + X = 5.
+  intros.
+  eexists; split.
+  - unfold "<". reflexivity.
+  - auto.
+Qed.
